More lenient pointer equality.
Pointer equality is now defined using absolute object offsets. The treatment
is similar to CompCert:

* Equality of pointers in the same object is defined provided the object has
  not been deallocated.
* Equality of pointers in different objects is defined provided both pointers
  have not been deallocated and both are strict (i.e. not end-of-array).

Thus, pointer equality is defined for all pointers that are not-end-of-array
and have not been deallocated. The following examples have defined behavior:

  int x, y;
  printf("%d\n", &x == &y);
  int *p = malloc(sizeof(int)), *q = malloc(sizeof(int));
  printf("%d\n", p == q);
  struct S { int a; int b; } s, *r = &s;
  printf("%d\n", &s.a + 1 == &(r->b));

The following not:

  int x, y;
  printf("%d\n", &x + 1 == &y);

tests/defined/pointer_comp.c
@@ -1,0 +1,9 @@
+
+int main() {
+  int x, y;
+  printf("%d\n", &x == &y);
+  int *p = malloc(sizeof(int)), *q = malloc(sizeof(int));
+  printf("%d\n", p == q);
+  struct S { int a; int b; } s, *r = &s;
+  printf("%d\n", &s.a + 1 == &(r->b));
+}
