tests/undefined/pointer_comp.c
@@ -1,0 +1,5 @@
+
+int main() {
+  int x, y;
+  printf("%d\n", &x + 1 == &y);
+}
